...

HouLean/OpenCL/Compiler/Main2.lean
@@ -8,6 +8,7 @@ open HouLean Lean Meta
 
 namespace HouLean.OpenCL.Compiler2
 
+
 structure Context where
   fvarMap : ExprMap String := {}
   usedNames : Std.HashMap String Nat := {}
@@ -329,24 +330,10 @@ run_meta
 --   logInfo m!"result:\n{e'}"
 
 
-/-- Gadget identity function that will stop `simp` from simplifying an expression.
 
-This is useful when the lhs of simp theorem appears on the rhs. You can wrap the occurence
-in `no_simp` an prevent simp from an infinite loop.
 
-The main use is for `simp` based compiler. For example for compiling to C we might define this
-function, which indicates that `spec` should be replaced with C function with the name `cfun`
-```
-def cFunction (spec : α) (cfun : String) : α := spec
-```
-Then we add the following simp theorem
-```
-theorem compile_sin : Float.sin = cFunction (no_simp Float.sin) "sin" := rfl
-```
-where we wrapped `Float.sin` in `no_simp` to preven this theorem to be applied again on the `spec`
-argument of `cFunction`.
- -/
-def no_simp {α : Sort u} (a : α) := a
+-- -- rewrite_rule : asdf = asdf
 
-simproc_decl no_simp_simproc (no_simp _) := fun e =>
-  return .done { expr := e }
+-- implemented_by (x y : Float) : x + y = x + y
+
+-- implemented_by (x : Float) : x.sin = sin(x)
