HouLean/OpenCL/Compiler/RewriteRules.lean
@@ -1,0 +1,199 @@
+import HouLean.OpenCL.Compiler.Grammar
+
+namespace HouLean.OpenCL.Compiler2
+
+/-- Gadget identity function that will stop `simp` from simplifying an expression.
+
+This is useful when the lhs of simp theorem appears on the rhs. You can wrap the occurence
+in `no_simp` an prevent simp from an infinite loop.
+
+The main use is for `simp` based compiler. For example for compiling to C we might define this
+function, which indicates that `spec` should be replaced with C function with the name `cfun`
+```
+def cFunction (spec : α) (cfun : String) : α := spec
+```
+Then we add the following simp theorem
+```
+theorem compile_sin : Float.sin = cFunction (no_simp Float.sin) "sin" := rfl
+```
+where we wrapped `Float.sin` in `no_simp` to preven this theorem to be applied again on the `spec`
+argument of `cFunction`. -/
+def no_simp {α : Sort u} (a : α) := a
+
+simproc_decl no_simp_simproc (no_simp _) := fun e =>
+  return .done { expr := e }
+
+
+def oclFunction' {type : Type} (spec : type) (name : String) (kind : OpenCLFunction.FunKind := .normal) : type := spec
+
+
+open Lean Meta Math
+
+structure ImplementedBy where
+  keys : Array DiscrTree.Key
+  argsToCompile : Array (Name × Nat)
+  lhs : Expr
+  rhs : TSyntax `oclExpr
+deriving Inhabited, BEq
+
+structure ImplementedByBuilder where
+  keys : Array DiscrTree.Key
+  lhs : Expr
+  syntaxBuilder : Name
+deriving Inhabited, BEq
+
+inductive SingleExtension where
+  | implementedBy (impl : ImplementedBy)
+  | implementedByBuilder (b : ImplementedByBuilder)
+deriving Inhabited
+
+/-- Enviroment extension that holds all necessary information for the APEX compiler. -/
+structure Extension where
+  implementedBy : DiscrTree ImplementedBy
+  implementedByBuilders : DiscrTree ImplementedByBuilder
+deriving Inhabited
+
+abbrev CompilerExt := SimpleScopedEnvExtension SingleExtension Extension
+
+initialize compilerExt : CompilerExt ←
+  registerSimpleScopedEnvExtension {
+    name := by exact decl_name%
+    initial := default
+    addEntry := fun es e =>
+      match e with
+      | .implementedBy impl =>
+        {es with implementedBy := es.implementedBy.insertCore impl.keys impl}
+      | .implementedByBuilder b =>
+        {es with implementedByBuilders := es.implementedByBuilders.insertCore b.keys b}
+  }
+
+
+partial def implementedBy (e : Expr) : MetaM (TSyntax `oclExpr) := do
+  let e ← instantiateMVars e
+  match e with
+  | .fvar id =>
+    let name ← id.getUserName
+    let id := mkIdent name
+    `(oclExpr| $id:ident)
+  | _ =>
+   -- let args := e.getAppArgs
+
+   let s := (compilerExt.getState (← getEnv)).implementedBy
+   let candidates ← s.getMatch e
+   for c in candidates do
+
+     let (args,_,body) ← lambdaMetaTelescope c.lhs
+
+     unless ← isDefEq body e do
+       continue
+
+     let mut compiledArgs : NameMap (TSyntax `oclExpr) := {}
+     for (n, i) in c.argsToCompile do
+       let some arg := args[i]?  | throwError m!"Can't apply {c.lhs} to {e}. Invalid argument index {i}!"
+       -- we might call `implementedBy` multiple times for one argument
+       -- this seems wasteful but I'm not expecting more
+       let arg ← implementedBy arg
+       compiledArgs := compiledArgs.insert n arg
+
+     -- todo: override for argList?
+
+     -- replace
+     let compiled ← c.rhs.raw.replaceM fun s =>
+       match s with
+       | `(oclExpr| $id:ident) =>
+         return compiledArgs.get? id.getId
+       | _ =>
+         return none
+
+     return ⟨compiled⟩
+
+   throwError "Don't know how to compile {e}!"
+
+open Lean Elab Term Command
+elab "impl_by" bs:bracketedBinder* " : " lhs:term  " ==> " rhs:oclExpr : command => do
+
+  runTermElabM fun ctx => do
+    elabBinders bs fun xs => do
+      let e ← elabTerm lhs none
+      -- let args := e.getAppArgs
+
+      let e ← mkLambdaFVars xs e >>= instantiateMVars
+      let ctx' := ctx.filter (fun c => e.containsFVar c.fvarId!)
+      let e ← mkLambdaFVars ctx' e >>= instantiateMVars
+
+      if e.hasMVar || e.hasFVar then
+        throwError s!"Bug in {decl_name%}, failed to build lhs expression!"
+
+      let args := ctx' ++ xs
+      -- collect identifiers that appear on the rhs
+      let argsToCompile : Array (Name × Nat) ←
+        (args.zip (.range args.size))
+        |>.filterMapM (fun (arg,i) => do
+          if arg.isFVar then
+            let name ← arg.fvarId!.getUserName
+            if rhs.raw.hasIdent name then
+              return some (name, i)
+          return none)
+
+      -- todo: add tracing
+      -- logInfo m!"lhs: {e}\nargs to compile: {argsToCompile}"
+
+      let (_,_,body) ← lambdaMetaTelescope e
+      let keys ← DiscrTree.mkPath body
+
+      -- let declName ← mkUniqueDeclName `implBy
+
+      let impl : ImplementedBy := {
+        keys := keys
+        argsToCompile := argsToCompile
+        lhs := e
+        rhs := rhs
+      }
+
+      compilerExt.add (.implementedBy impl)
+
+
+open Lean Elab Term Command Qq
+elab "impl_by" bs:bracketedBinder* " : " lhs:term  " ==> " "do" rhs:doElem* : command => do
+
+  runTermElabM fun ctx => do
+    elabBinders bs fun xs => do
+      let e ← elabTerm lhs none
+
+      let e ← mkLambdaFVars xs e >>= instantiateMVars
+      let ctx' := ctx.filter (fun c => e.containsFVar c.fvarId!)
+      let e ← mkLambdaFVars ctx' e >>= instantiateMVars
+
+
+      let decls ← (ctx'++xs).mapM (fun x => do
+        return (← x.fvarId!.getUserName, .default, fun _ => pure q(Expr)))
+      let builder ← liftM <|
+        withLocalDecls decls fun ys => do
+          let rhs ← elabTermAndSynthesize (← `(term| do $[$rhs:doElem]*)) q(MetaM (TSyntax `oclExpr))
+          mkLambdaFVars ys rhs
+
+      let builderType ← inferType builder >>= instantiateMVars
+      let builderDeclName ← mkUniqueDeclName `implStxBuilder
+
+      let decl : Declaration := .defnDecl {
+        name := builderDeclName
+        levelParams := []
+        type := builderType
+        value := builder
+        hints := .regular builder.approxDepth
+        safety := .safe
+      }
+
+      addAndCompile decl
+
+      let (_,_,body) ← lambdaMetaTelescope e
+      let keys ← DiscrTree.mkPath body
+
+      let b : ImplementedByBuilder := {
+        keys := keys
+        lhs := e
+        syntaxBuilder := builderDeclName
+      }
+
+      compilerExt.add (.implementedByBuilder b)
+      logInfo m!"script:\n{rhs}"
