HouLean/OpenCL/Reference/Operators.lean
@@ -1,0 +1,103 @@
+import HouLean.OpenCL.Compiler.RewriteRules
+
+open HouLean OpenCL Compiler Math
+
+namespace HouLean.OpenCL
+
+variable {R} {m n : Nat} (x y z : R) (u v : Vector R n) (a b : Bool)
+
+-- '+'
+impl_by [AtomicOpenCLType R] [Add R] : x + y ==> x + y
+impl_by [AtomicOpenCLType R] [AllowedVectorSize n] [Add R] : u + v ==> u + v
+
+-- '-'
+impl_by [AtomicOpenCLType R] [Sub R] : x - y ==> x - y
+impl_by [AtomicOpenCLType R] [AllowedVectorSize n] [Sub R] : u - v ==> u - v
+
+impl_by [AtomicOpenCLType R] [Neg R] : - x ==> - x
+impl_by [AtomicOpenCLType R] [AllowedVectorSize n] [Neg R] : - u ==> - u
+
+-- '*'
+impl_by [AtomicOpenCLType R] [Mul R] : x * y ==> x * y
+impl_by [AtomicOpenCLType R] [AllowedVectorSize n] [Mul R] : x * u ==> x * u
+
+-- '%'
+impl_by [AtomicOpenCLType R] [Mod R] : x % y ==> x % y
+
+-- '/'
+impl_by [AtomicOpenCLType R] [Div R] : x / y ==> x / y
+
+
+-- '--'
+
+-- '++'
+
+-- '=='
+impl_by : a == b ==> a == b
+impl_by [AtomicOpenCLType R] [BEq R] : x == y ==> x == y
+impl_by [AtomicOpenCLType R] [AllowedVectorSize n] [BEq R] : u == v ==> u == v
+
+impl_by : decide (b = true) ==> b
+impl_by : decide (b = false) ==> !b
+impl_by : decide (a = b) ==> a == b
+impl_by [AtomicOpenCLType R] [DecidableEq R] : decide (x = y) ==> a == b
+impl_by [AtomicOpenCLType R] [AllowedVectorSize n] [DecidableEq R] : decide (u = v) ==> u == v
+
+-- `!=`
+impl_by (a b : Bool) : a != b ==> a != b
+impl_by [AtomicOpenCLType R] [BEq R] : x != y ==> x != y
+impl_by [AtomicOpenCLType R] [AllowedVectorSize n] [BEq R] : u != v ==> u != v
+
+-- '&'
+impl_by [AtomicOpenCLType R] [AndOp R] : x &&& y ==> x & y
+
+-- '~'
+
+-- '^'
+impl_by [AtomicOpenCLType R] [AndOp R] : x &&& y ==> x & y
+
+-- '>'
+
+-- '<'
+
+-- '>='
+
+-- '<='
+
+-- '|'
+impl_by [AtomicOpenCLType R] [OrOp R] : x ||| y ==> x | y
+
+-- '!'
+impl_by : !a ==> !a
+impl_by : decide (¬a) ==> !a
+
+
+
+-- '&&'
+impl_by (a b : Bool) : a && b ==> a && b
+example {P Q} [Decidable P] [Decidable Q] : decide (P ∧ Q) = decide P && decide Q := sorry_proof
+
+-- '||'
+impl_by (a b : Bool) : a || b ==> a || b
+example {P Q} [Decidable P] [Decidable Q] : decide (P ∨ Q) = decide P || decide Q := sorry_proof
+
+
+-- '?:'
+
+-- '>>'
+impl_by [AtomicOpenCLType R] [ShiftRight R] : x >>> y ==> x >> y
+
+-- '<<'
+impl_by [AtomicOpenCLType R] [ShiftLeft R]  : x <<< y ==> x << y
+
+-- '='
+
+-- ','
+
+-- 'op='
+
+
+-- 'sizeof'
+
+
+impl_by (b : Bool) : decide (b = true) ==> b
