Tests/OpenCL/RewriteRules.lean
@@ -1,0 +1,201 @@
+import HouLean.OpenCL.Compiler.RewriteRules
+
+
+open HouLean OpenCL Compiler Math
+
+
+
+variable {R} {m n : Nat}
+set_option pp.funBinderTypes true
+
+variable (x y z : R) (u v : Vector R n)
+
+-- Operators And Qualifiers
+
+-- plus
+impl_by [AtomicOpenCLType R] [Add R] : x + y ==> x + y
+impl_by [AtomicOpenCLType R] [AllowedVectorSize n] [Add R] : u + v ==> u + v
+
+-- minus
+impl_by [AtomicOpenCLType R] [Sub R] : x - y ==> x - y
+impl_by [AtomicOpenCLType R] [AllowedVectorSize n] [Sub R] : u - v ==> u - v
+
+impl_by [AtomicOpenCLType R] [Neg R] : - x ==> - x
+impl_by [AtomicOpenCLType R] [AllowedVectorSize n] [Neg R] : - u ==> - u
+
+-- mul
+impl_by [AtomicOpenCLType R] [Mul R] : x * y ==> x * y
+impl_by [AtomicOpenCLType R] [AllowedVectorSize n] [Mul R] : x * u ==> x * u
+
+-- div
+impl_by [AtomicOpenCLType R] [Div R] : x / y ==> x / y
+
+-- '--'
+-- missing
+
+-- '++'
+-- missing
+
+-- '=='
+impl_by (a b : Bool) : a == b ==> a == b
+impl_by [AtomicOpenCLType R] [BEq R] : x == y ==> x == y
+impl_by [AtomicOpenCLType R] [AllowedVectorSize n] [BEq R] : u == v ==> u == v
+
+-- `!=`
+impl_by (a b : Bool) : a != b ==> a != b
+impl_by [AtomicOpenCLType R] [BEq R] : x != y ==> x != y
+impl_by [AtomicOpenCLType R] [AllowedVectorSize n] [BEq R] : u != v ==> u != v
+
+-- '&'
+impl_by [AtomicOpenCLType R] [AndOp R] : x &&& y ==> x & y
+
+
+
+impl_by (b : Bool) : decide (b = true) ==> b
+
+
+impl_by [AtomicOpenCLType R] [Mod R] : x % y ==> x % y
+impl_by [AtomicOpenCLType R] [Mod R] : x % y ==> x % y
+
+impl_by [AtomicOpenCLType R] [ShiftRight R] : x >>> y ==> x >> y
+impl_by [AtomicOpenCLType R] [ShiftLeft R]  : x <<< y ==> x << y
+impl_by [AtomicOpenCLType R] [AndOp R]      : x &&& y ==> x & y
+impl_by [AtomicOpenCLType R] [OrOp R]       : x ||| y ==> x | y
+
+impl_by (b : Bool) : decide (b = true) ==> b
+impl_by (b : Bool) : decide (b = false) ==> !b
+impl_by (a b : Bool) : a && b ==> a && b
+impl_by (a b : Bool) : a || b ==> a || b
+
+
+
+
+impl_by (P Q : Prop) [Decidable P] [Decidable Q] : decide (P ∧ Q) ==> P && Q
+
+section Math
+open Math
+
+variable [FloatType R] (x y : R)
+
+impl_by : sin x ==> sin(x)
+impl_by : cos x ==> cos(x)
+impl_by : exp x ==> exp(x)
+impl_by : atan2 y x ==> atan2(y, x)
+
+
+end Math
+
+-- todo: how to generalize this ???
+section
+variable (x y z w : Float32)
+impl_by :     #v[x,y] ==> (float2){x,y}
+impl_by :   #v[x,y,z] ==> (float3){x,y,z}
+impl_by : #v[x,y,z,w] ==> (float4){x,y,z,w}
+end
+
+section
+variable (x y z w : Float64)
+impl_by :     #v[x,y] ==> (double2){x,y}
+impl_by :   #v[x,y,z] ==> (double3){x,y,z}
+impl_by : #v[x,y,z,w] ==> (double4){x,y,z,w}
+end
+
+section
+variable (x y z w : Int)
+impl_by :     #v[x,y] ==> (int2){x,y}
+impl_by :   #v[x,y,z] ==> (int3){x,y,z}
+impl_by : #v[x,y,z,w] ==> (int4){x,y,z,w}
+end
+
+section
+variable (x y z w : Nat)
+impl_by :     #v[x,y] ==> (uint2){x,y}
+impl_by :   #v[x,y,z] ==> (uint3){x,y,z}
+impl_by : #v[x,y,z,w] ==> (uint4){x,y,z,w}
+end
+
+
+-- not sure if this is a way to go for types, but it looks nice ...
+-- but for structures we want to do it automatically
+-- the only exception are matrices whose OpenCL implementation does not match
+impl_by : Float32 ==> float
+impl_by : Float64 ==> double
+impl_by :     Nat ==> uint
+impl_by :     Int ==> int
+impl_by :  UInt16 ==> ushort
+impl_by :  UInt32 ==> uint
+impl_by :  UInt64 ==> ulong
+impl_by :   Int16 ==> short
+impl_by :   Int32 ==> int
+impl_by :   Int64 ==> long
+
+
+open Lean Meta Qq Compiler2
+run_meta
+  let e := q(fun x y : Float => x + atan2 (x + y) (sin (x + y)))
+  lambdaTelescope e fun _ body => do
+  let stx ← implementedBy body
+  logInfo stx
+
+open Lean Meta Qq Compiler2
+run_meta
+  let e := q(fun x y : Float => #v[x+x, x*x, x/y])
+  lambdaTelescope e fun _ body => do
+  let stx ← implementedBy body
+  logInfo stx
+
+
+open Lean Meta
+def identFromString (s : String) : Ident := mkIdent (Name.mkSimple s)
+
+
+impl_by [AtomicOpenCLType R] : Vector R n ==> do
+  let type ← implementedBy R
+  let typeName := toString type
+  let id := identFromString (typeName ++ toString n)
+  return ← `(oclExpr| $id:ident)
+
+impl_by [t : AtomicOpenCLType R] : Matrix R m n ==> do
+  let type ← implementedBy R
+  let typeName := toString type
+  let id := identFromString ("matrix" ++ typeName ++ toString m ++ toString n)
+  return ← `(oclExpr| $id:ident)
+
+impl_by : Int ==> int
+
+-- impl_by {α β : Type} :
+--   α × β
+--   ==>
+--   structure {
+--     α fst;
+--     β snd;
+--   }
+
+
+theorem float_add (x y : Float) : x + y = ocl%( x + y ) := sorry_proof
+theorem atomic_type_add {R} [AtomicOpenCLType R] [Add R] [Inhabited R] (x y : R) :
+    x + y = ocl%( x + y ) := sorry_proof
+theorem float_type_sin {R} [FloatType R] (x : R) :
+    sin x = ocl%( sin(x) ) := sorry_proof
+
+-- theorem vector_mk (ls : List α) (h : ls.toArray.size = n) :
+--     Vector.mk ls.toArray h = ocl%( (α){ ls,* } ) := sorry_proof
+
+theorem float_ocl : Float32 = ocl%( float ) := sorry_proof
+theorem double_ocl : Float64 = ocl%( double ) := sorry_proof
+theorem nat_ocl : Nat = ocl%( uint ) := sorry_proof
+theorem int_ocl : Int = ocl%( int ) := sorry_proof
+-- theorem prod_ocl {α β : Type} :
+--   (α × β)
+--   =
+--   ocl%( structure {
+--            α fst;
+--            β snd;
+--         }) := sorry_proof
+
+
+theorem float_add' (x y : Float) : x + y = oclFunction' (no_simp (·+·)) " + " .infix x y := by rfl
+theorem atomic_type_add' {R} [AtomicOpenCLType R] [Add R] (x y : R) :
+    x + y = oclFunction' (no_simp (·+·)) " + " .infix x y := by rfl
+theorem float_type_sin' {R} [FloatType R] (x : R) :
+    sin x = (oclFunction' (no_simp sin) "sin") x := by rfl
